# Chapter 1.2: Count of Elements

## Introduction

Theorem 1 (**Principle of Inclusion and Exclusion** formula):

$$|A \cup B| = |A| + |B| - |A \cap B|$$

or, more generally:

$$|A_1 \cup ... \cup A_n| = \sum_{i}^{} |A_i| - \sum_{i<j}^{} |A_i \cap A_j| + \sum_{i<j<k}^{} |A_i \cap A_j \cap A_k| - ...$$

---

**Characteristic function**:

$$\chi_{X} : \forall X \subset U \implies (e \in X \implies \chi_{X}(e) = 1) \land (e \in (U \setminus X) \implies \chi_{X}(e) = 0)$$

---

**One-to-one correspondence**:

Two sets $A$ and $B$ are said to be equivalent if there is some [bijection](https://en.wikipedia.org/wiki/Bijection) from $A$ onto $B$.

---

## 15

Prove:

$$|A_1 \triangle ... \triangle A_n| = \sum_{i}^{} |A_i| - 2^{1}\sum_{i<j}^{} |A_i \cap A_j| + 2^{2}\sum_{i<j<k}^{} |A_i \cap A_j \cap A_k| - ...$$

---

Assume $U : \forall A_i \in U, i \in \{1..n\}$.

Original formula could then be rewritten as follows using characteristic functions [15-1]:

$$\chi_{A_1 \triangle ... \triangle A_n} = \sum_{i}^{} \chi_{A_i} - 2^{1}\sum_{i<j}^{} \chi_{A_i} \chi_{A_j} + 2^{2}\sum_{i<j<k}^{} \chi_{A_i} \chi_{A_j} \chi_{A_k} - ...$$

Proof by induction:

* Induction base: $\chi_{A_1 \triangle A_2} = \chi_{(A \cup B) \setminus (A \cap B)} = \chi_{A \cup B} - \chi_{A \cap B} = (\chi_{A_1} + \chi_{A_2} - \chi_{A_1} \chi_{A_2}) - (\chi_{A_1} \chi_{A_2}) = \chi_{A_1} + \chi_{A_2} - 2\chi_{A_1} \chi_{A_2}$.
* Induction step: assume formula is true for $n-1$, in this case using associativity property of symmetric difference the original formula could be rewritten as $\chi_{(A_1 \triangle ... \triangle A_{n-1}) \triangle A_n}$. Assume $B = A_1 \triangle ... \triangle A_{n-1}$: $\chi_{B \triangle A_n} = \chi_{B} + \chi_{A_n} - 2\chi_{B} \chi_{A_n} = \chi_{A_n} + (\sum_{i}^{} \chi_{A_i} - 2^{1}\sum_{i<j}^{} \chi_{A_i} \chi_{A_j} + 2^{2}\sum_{i<j<k}^{} \chi_{A_i} \chi_{A_j} \chi_{A_k} - ...) - 2 \chi_{A_n}(\sum_{i}^{} \chi_{A_i} - 2^{1}\sum_{i<j}^{} \chi_{A_i} \chi_{A_j} + 2^{2}\sum_{i<j<k}^{} \chi_{A_i} \chi_{A_j} \chi_{A_k} - ...)$ which yields formula [15-1] which in its turn yields original formula. $\blacksquare$

$$A \not\subset B$$

# 16

# 17

# 18

# 19

# 20

# 21

# 22

# 23

# 24

# 25
